src/3d/Main.fst
@@ -262,7 +262,7 @@ let go () : ML unit =
   let _ = Batch.postprocess_fst
         (Options.get_clang_format ())
         (Options.get_clang_format_executable ())
-        (Options.get_skip_makefiles ())
+        (Options.get_skip_c_makefiles ())
         (Options.get_cleanup ())
         (Options.get_no_everparse_h ())
         (Options.get_save_hashes ())
