src/3d/Options.fsti
@@ -28,7 +28,7 @@ val get_clang_format_executable : unit -> ML string
 
 val get_cleanup : unit -> ML bool
 
-val get_skip_makefiles : unit -> ML bool
+val get_skip_c_makefiles : unit -> ML bool
 
 val get_no_everparse_h : unit -> ML bool
 
